Achieved proofs of termination of simply typed lc

LambdaCalculus.v
@@ -1,5 +1,12 @@
 Require Import Arith.
 
+Function iterate {X : Type} (n : nat) (f : X -> X) (x0 : X) :=
+  match n with
+    | 0 => x0
+    | S n => f (iterate n f x0)
+  end.
+
+
 Inductive term : Set :=
 | TVar : nat -> term
 | TApp : term -> term -> term
@@ -71,6 +78,7 @@ Inductive beta_reduction : term -> term -> Prop :=
             beta_reduction (TApp (TAbstr u) v) ([0 := v]u)
 
 where "u '-->' v" := (beta_reduction u v).
+
 
 
 Section Confluence.
@@ -356,6 +364,13 @@ Module Parallel.
 
   Hint Constructors par_reduction.
 
+  Definition par_star :=
+    RStar term par_reduction.
+
+
+  Notation "u '==>*' v" := (par_star u v) (at level 20).
+
+
   Lemma beta_implies_par :
     forall (a b : term),
       a --> b -> a ==> b.
@@ -381,6 +396,20 @@ Module Parallel.
       apply b_app1_star. apply b_abstr_star. assumption.
       apply b_app2_star. assumption.
       apply clos_rt1n_step. apply b_red.
+  Qed.
+
+  Lemma par_star_equiv_beta_star :
+    forall (a b : term),
+      a ==>* b <-> a -->* b.
+  Proof.
+    intros a b.
+    split.
+    - intros H. induction H.
+      + apply rt1n_refl.
+      + apply rstar_trans with y. apply par_implies_beta_star. assumption. assumption.
+    - intros H. induction H.
+      + apply rt1n_refl.
+      + apply rt1n_trans with y. apply beta_implies_par. assumption. assumption.
   Qed.
 
   Lemma par_refl :
@@ -654,4 +683,1278 @@ Module Parallel.
        split ; apply r_step ; apply subst_par...
   Qed.
 
+  Theorem par_confluent : confluent term par_reduction.
+  Proof. apply strongly_confluent_confluent.
+         apply par_strongly_confluent.
+  Qed.
+
 End Parallel.
+
+
+
+
+Theorem beta_confluent :
+  confluent term beta_reduction.
+Proof.
+  intros x y z Hy Hz.
+  apply Parallel.par_star_equiv_beta_star in Hy.
+  apply Parallel.par_star_equiv_beta_star in Hz.
+  elim (Parallel.par_confluent x y z Hy Hz).
+  intros w [Hyw Hzw].
+  apply Parallel.par_star_equiv_beta_star in Hyw.
+  apply Parallel.par_star_equiv_beta_star in Hzw.
+  exists w. auto.
+Qed.
+
+
+Lemma rescope_app_congr :
+  forall (s u1 u2 : term) (n : nat),
+    rescope s n = TApp u1 u2 ->
+    exists (s1 : term),
+      exists (s2 : term),
+        s = TApp s1 s2 /\ rescope s1 n = u1 /\ rescope s2 n = u2.
+Proof.
+  intros s u1 u2 n H.
+  destruct s.
+  - simpl in H. destruct (leb n n0) ; inversion H.
+  - simpl in H. inversion H.
+    exists s1. exists s2. split ; [idtac | split] ; reflexivity.
+  - simpl in H. inversion H.
+Qed.
+
+
+Lemma rescope_abstr_congr :
+  forall (s u1 : term) (n : nat),
+    rescope s n = TAbstr u1 ->
+    exists (s1 : term), s = TAbstr s1 /\ rescope s1 (S n) = u1.
+Proof.
+  intros s u1 n H.
+  destruct s ; simpl in H.
+  - destruct (leb n n0) ; inversion H.
+  - inversion H.
+  - inversion H. exists s. split ; reflexivity.
+Qed.
+
+Lemma rescope_reduction :
+  forall (u w : term) (n : nat),
+    rescope u n --> w ->
+    exists (v : term), w = rescope v n /\ u --> v.
+Proof.
+  intros u w n Hw.
+  remember (rescope u n). generalize dependent n. generalize u.
+  induction Hw.
+  - intros s n Heq.
+    symmetry in Heq.
+    assert (G := rescope_app_congr s t1 t2 n Heq).
+    destruct G as [s1 [s2 [Geq [Gu1 Gu2]]]].
+    symmetry in Gu1.
+    destruct (IHHw s1 n Gu1) as [v1 [K1 Kr]].
+    exists (TApp v1 s2). split.
+    simpl. rewrite Gu2. rewrite K1. reflexivity.
+    rewrite Geq. apply b_app1. assumption.
+  - intros s n Heq.
+    symmetry in Heq.
+    assert (G := rescope_app_congr s t1 t2 n Heq).
+    destruct G as [s1 [s2 [Geq [Gu1 Gu2]]]].
+    symmetry in Gu2.
+    destruct (IHHw s2 n Gu2) as [v2 [K2 Kr]].
+    exists (TApp s1 v2). split.
+    simpl. rewrite Gu1. rewrite K2. reflexivity.
+    rewrite Geq. apply b_app2. assumption.
+  - intros s n Heq.
+    symmetry in Heq.
+    assert (G := rescope_abstr_congr s u0 n Heq).
+    destruct G as [s1 [Geq Gu0]].
+    symmetry in Gu0.
+    destruct (IHHw s1 (S n) Gu0) as [v [K0 Kr]].
+    exists (TAbstr v). split.
+    * simpl. rewrite K0. reflexivity.
+    * rewrite Geq. apply b_abstr. assumption.
+  - intros u1 n Heq.
+    symmetry in Heq.
+    destruct (rescope_app_congr u1 (TAbstr u0) v n Heq)
+      as [abs1 [arg1 [Geq [G1 G2]]]].
+    destruct (rescope_abstr_congr _ _ _ G1) as [abs2 [Keq K2]].
+    rewrite Geq. exists ([0 := arg1]abs2).
+    rewrite <- Parallel.rescope_factorization'.
+    rewrite G2. rewrite K2. split. reflexivity. rewrite Keq.
+    apply b_red. omega.
+Qed.
+
+Lemma rescope_congr :
+  forall (u v : term) (n : nat), u --> v -> (rescope u n) --> (rescope v n).
+Proof.
+  intros u v n H. generalize dependent n.
+  induction H.
+  - intros n. simpl. apply b_app1. apply IHbeta_reduction.
+  - intros n. simpl. apply b_app2. apply IHbeta_reduction.
+  - intros n. simpl. apply b_abstr. apply IHbeta_reduction.
+  - intros n. simpl. rewrite <- Parallel.rescope_factorization'.
+    apply b_red. omega.
+Qed.
+
+
+Lemma subst_reduction :
+  forall (u u' v : term) (n : nat), u --> u' -> [n := v]u --> [n := v]u'.
+Proof.
+  intros u. induction u.
+  - intros u' v k Hcontra. inversion Hcontra.
+  - intros u' v k H. inversion H ; subst.
+    + simpl. apply b_app1. apply IHu1. assumption.
+    + simpl. apply b_app2. apply IHu2. assumption.
+    + rewrite Parallel.subst_commutator. simpl.
+      apply b_red. omega.
+  - intros u' v n Hu. inversion Hu. simpl.
+    apply b_abstr. apply IHu. assumption.
+Qed.
+
+Lemma subst_abstr_inversion :
+  forall (u v : term) (p k : nat),
+    TAbstr u = [p := TVar k]v -> exists (w : term),  v = TAbstr w.
+Proof.
+  intros u v. generalize dependent u.
+  induction v ; simpl.
+  - intros u p s contra. destruct (nat_compare p n) ; inversion contra.
+  - intros u p s contra. inversion contra.
+  - intros u p k H. exists v. reflexivity.
+Qed.
+
+
+Lemma subst_reduction_inversion :
+  forall (u v : term) (p n : nat),
+    [p := TVar n]u --> v ->
+    exists (u' : term), v = [p := TVar n]u' /\ u --> u'.
+Proof.
+  intros u. induction u ; simpl.
+  - intros v p k Hcontra. destruct (nat_compare p n) ; inversion Hcontra.
+  - intros v p k H. inversion H ; subst ; simpl.
+    + destruct (IHu1 _ _ _ H3) as [w [Hw Hr]].
+      exists (TApp w u2). split. rewrite Hw. reflexivity.
+      apply b_app1. assumption.
+    + destruct (IHu2 _ _ _ H3) as [w [Hw Hr]].
+      exists (TApp u1 w). split. rewrite Hw. reflexivity.
+      apply b_app2. assumption.
+    + destruct (subst_abstr_inversion _ _ _ _ H1) as [w Hw].
+      exists ([0 := u2]w). rewrite Parallel.subst_commutator.
+      rewrite Hw in H1. simpl in H1. inversion H1.
+      split. reflexivity. rewrite Hw. apply b_red. omega.
+  - intros v p k H. inversion H ; subst ; simpl.
+    destruct (IHu _ _ _ H1) as [w [Hw Hr]].
+    exists (TAbstr w). rewrite Hw. split. reflexivity. apply b_abstr. assumption.
+Qed.
+
+
+
+(*
+Module LeftmostUppermost.
+  Require Import List.
+  Open Scope list_scope.
+
+  Inductive as_head_term : Set :=
+  | ht_normal : forall (i : nat), as_head_term
+  | ht_redex : forall (u v : term), as_head_term.
+
+  Function head_term_value (t : as_head_term) :=
+    match t with
+      | ht_normal i => TVar i
+      | ht_redex u v => TApp (TAbstr u) v
+    end.
+
+  Fixpoint head_abstractions term :=
+    match term with
+      | TVar _ | TApp _ _ => 0
+      | TAbstr u => S (head_abstractions u)
+    end.
+
+  Fixpoint head_term term :=
+    match term with
+      | TVar i => ht_normal i
+      | TApp u v =>
+        match u with
+          | TAbstr u' => ht_redex u' v
+          | _ => head_term u
+        end
+      | TAbstr u => head_term u
+    end.
+
+  Fixpoint other_terms term :=
+    match term with
+      | TVar i => nil
+      | TApp u v =>
+        match u with
+          | TAbstr _ => nil
+          | _ => other_terms u ++ (v :: nil)
+        end
+      | TAbstr u => other_terms u
+    end.
+
+  Fixpoint all_terms term :=
+    match term with
+      | TVar i => (TVar i :: nil)
+      | TApp u v =>
+        match u with
+          | TAbstr _ => u :: v :: nil
+          | _ => all_terms u ++ (v :: nil)
+        end
+      | TAbstr u => all_terms u
+    end.
+
+ Function term_of_simili_head_form nabs t ot :=
+   iterate nabs TAbstr (fold_left TApp ot t).
+
+ Function term_of_head_form nabs ht ot :=
+   term_of_simili_head_form nabs (head_term_value ht) ot.
+
+
+
+  Lemma head_term_app_app :
+    forall (u v w : term),
+      head_term (TApp (TApp u v) w) = head_term (TApp u v).
+  Proof. reflexivity. Qed.
+
+  Lemma other_terms_app_app :
+    forall (u v w : term),
+      other_terms (TApp (TApp u v) w) = other_terms (TApp u v) ++ (w :: nil).
+  Proof. reflexivity. Qed.
+
+  Lemma term_of_simili_hf_app :
+    forall (l : list term) (t : term) (h : term),
+      term_of_simili_head_form 0 h (l ++ (t :: nil)) =
+      TApp (term_of_simili_head_form 0 h l) t.
+  Proof.
+    intros l t h. induction l.
+    - reflexivity.
+    - unfold term_of_simili_head_form. apply fold_left_app.
+  Qed.
+
+  Lemma term_of_hf_app :
+    forall (l : list term) (t : term) (h : as_head_term),
+      term_of_head_form 0 h (l ++ (t :: nil)) =
+      TApp (term_of_head_form 0 h l) t.
+  Proof.
+    intros l t h.
+    unfold term_of_head_form. apply term_of_simili_hf_app.
+  Qed.
+
+
+  Lemma term_hf_id :
+    forall (u : term),
+      term_of_head_form (head_abstractions u) (head_term u) (other_terms u) = u.
+  Proof.
+    intros u. induction u.
+    - unfold term_of_head_form. reflexivity.
+    - generalize dependent u2. destruct u1.
+      + reflexivity.
+      + intros u2 IHu2.
+        rewrite head_term_app_app.
+        rewrite other_terms_app_app.
+        simpl (head_abstractions _).
+        rewrite term_of_hf_app.
+        simpl (head_abstractions _) in IHu1. rewrite IHu1. reflexivity.
+      + intros u2 IHu2. unfold term_of_head_form. reflexivity.
+    - unfold term_of_head_form. unfold term_of_simili_head_form.
+      unfold term_of_head_form in IHu. unfold term_of_simili_head_form in IHu.
+      simpl. rewrite IHu. reflexivity.
+  Qed.
+
+  Lemma head_abstractions_apps :
+    forall (ht : term) (ot : list term),
+      ot <> nil ->
+      head_abstractions (fold_left TApp ot ht) = 0.
+  Proof.
+    intros ht ot. generalize dependent ht.
+    induction ot ; intros ht Habs.
+    - contradict Habs. reflexivity.
+    - simpl. destruct ot.
+      + reflexivity.
+      + apply IHot. intros H. discriminate H.
+  Qed.
+
+  Lemma head_term_abs :
+    forall (nabs : nat) (u : term),
+      head_term (iterate nabs TAbstr u) = head_term u.
+  Proof. intros nabs. induction nabs ; intros u.
+         - reflexivity.
+         - simpl. apply IHnabs.
+  Qed.
+
+  Lemma head_term_app :
+    forall (ot : list term) (ht : as_head_term),
+      head_term (fold_left TApp ot (head_term_value ht)) = ht.
+  Proof. intros ot. induction ot using rev_ind.
+         - intros ht. destruct ht ; reflexivity.
+         - intros ht.
+           rewrite fold_left_app. simpl. rewrite IHot.
+           induction ot using rev_ind.
+           + simpl. destruct ht ; reflexivity.
+           + rewrite fold_left_app. reflexivity.
+  Qed.
+
+  Lemma other_terms_abs :
+    forall (nabs : nat) (u : term),
+      other_terms (iterate nabs TAbstr u) = other_terms u.
+  Proof.
+    intros nabs. induction nabs ; auto.
+  Qed.
+
+  Lemma other_terms_app :
+    forall (ot : list term) (ht : as_head_term),
+      other_terms (fold_left TApp ot (head_term_value ht)) = ot.
+  Proof.
+    induction ot using rev_ind.
+    - intros ht. destruct ht ; reflexivity.
+    - intros ht. rewrite fold_left_app. simpl. rewrite IHot.
+      induction ot using rev_ind.
+      + simpl. destruct ht ; reflexivity.
+      + rewrite fold_left_app. reflexivity.
+  Qed.
+
+  Lemma hf_term_id :
+    forall (nabs : nat) (ht : as_head_term) (ot : list term),
+      head_abstractions (term_of_head_form nabs ht ot) = nabs /\
+      head_term (term_of_head_form nabs ht ot) = ht /\
+      other_terms (term_of_head_form nabs ht ot) = ot.
+  Proof.
+    intros nabs ht ot.
+    split ; [ idtac | split].
+    - induction nabs.
+      + unfold term_of_head_form. simpl.
+        induction ot.
+        * simpl. destruct ht ; reflexivity.
+        * apply head_abstractions_apps. intro H. discriminate H.
+      + simpl. unfold term_of_head_form in IHnabs.
+        unfold term_of_simili_head_form in IHnabs.
+        rewrite IHnabs. reflexivity.
+    - unfold term_of_head_form.
+      unfold term_of_simili_head_form.
+      rewrite head_term_abs.
+      rewrite head_term_app. reflexivity.
+    - unfold term_of_head_form.
+      unfold term_of_simili_head_form.
+      rewrite other_terms_abs.
+      rewrite other_terms_app. reflexivity.
+  Qed.
+
+
+  Lemma hf_term_id_abs :
+    forall (nabs : nat) (ht : as_head_term) (ot : list term),
+      head_abstractions (term_of_head_form nabs ht ot) = nabs.
+  Proof. intros nabs ht ot. destruct (hf_term_id nabs ht ot) as [H _ _].
+         assumption. Qed.
+
+  Inductive head_reduction : term -> term -> Prop :=
+  | hd_beta : forall (nabs : nat) (u v : term) (ot : list term),
+                head_reduction (term_of_head_form nabs (ht_redex u v) ot)
+                               (term_of_simili_head_form nabs ([0 := v]u) ot).
+
+
+  Definition head_reduction_star := RStar term head_reduction.
+
+  Lemma head_reduction_app :
+    forall (u1 u1' u2 : term),
+      head_reduction u1 u1' -> head_abstractions u1 = 0 ->
+      head_reduction (TApp u1 u2) (TApp u1' u2).
+  Proof.
+    intros u1 u1' u2 H Habs.
+    inversion H.
+    rewrite <- H0 in Habs.
+    rewrite hf_term_id_abs in Habs. subst.
+    rewrite <- term_of_hf_app.
+    rewrite <- term_of_simili_hf_app.
+    apply hd_beta.
+  Qed.
+
+  Lemma head_reduction_star_app :
+    forall (u1 u1' u2 : term),
+      head_reduction_star u1 u1' -> head_abstractions u1 = 0 ->
+      head_reduction_star (TApp u1 u2) (TApp u1' u2).
+  Proof.
+    intros u1 u1' u2 H.
+    induction H ; intros G.
+    - apply rt1n_refl.
+    - apply rt1n_trans with (TApp y u2).
+      apply head_reduction_app ; assumption.
+
+
+  Inductive leftmost_uppermost : term -> term -> Prop :=
+  | lu_red : forall (u v w: term),
+               head_reduction_star u v ->
+               on_components (all_terms v) (all_terms w) ->
+               leftmost_uppermost u w
+  | lu_var : forall (i : nat),  leftmost_uppermost (TVar i) (TVar i)
+  with on_components : list term -> list term -> Prop :=
+       | oc_nil : on_components nil nil
+       | oc_cons : forall (a b : term) (la lb : list term), leftmost_uppermost a b -> on_components la lb -> on_components (a :: la) (b :: lb).
+
+
+  Scheme lu_on_components_ind := Induction for leftmost_uppermost Sort Prop
+    with on_components_lu_ind := Induction for on_components Sort Prop.
+
+  Combined Scheme lu_mutind from lu_on_components_ind.
+
+
+  Lemma all_terms_non_empty : forall (u : term), nil <> all_terms u.
+  Proof.
+    intros u. induction u.
+    - simpl. intros G. discriminate G.
+    - simpl. destruct u1 ; try apply app_cons_not_nil.
+      + intros G. discriminate G.
+    - simpl. apply IHu.
+  Qed.
+
+  Lemma head_form_induction :
+    forall (P : term -> Prop),
+      (forall (i : nat),  P (TVar i)) ->
+      (forall (u : list term) -> nabs u > 0 ->
+
+  Lemma all_term_head_tail :
+    forall (u : term),
+    exists (hd : term), exists (tl : list term),
+                          all_terms u = hd :: tl.
+  Proof.
+    intros u.
+    destruct (all_terms u) eqn:Eq.
+    - symmetry in Eq. exfalso.
+      contradict (all_terms_non_empty u Eq).
+    - exists t. exists l. reflexivity.
+  Qed.
+
+  (*
+  Lemma lu_app :
+    forall (u1 u1' u2 u2' : term),
+      leftmost_uppermost u1 u1' -> leftmost_uppermost u2 u2' ->
+      leftmost_uppermost (TApp u1 u2) (TApp u1' u2').
+  Proof.
+    intros u1 u1' u2 u2' G1. generalize dependent u2'. generalize dependent u2.
+    induction G1.
+    - intros u2 u2' G2.
+      destruct (all_term_head_tail (TApp u u2)) as [x [y Hxy]].
+      eapply lu_red.
+      + apply rt1n_refl.
+      + apply Hxy.
+      +
+*)
+  Lemma lu_refl_n :
+    forall (u : term),
+      leftmost_uppermost u u.
+  Proof.
+    intros u.
+    remember (all_terms u). generalize dependent u.
+    induction l ; intros u Heql.
+    - exfalso. eapply all_terms_non_empty. apply Heql.
+    -
+    - apply lu_var.
+    -
+    - destruct (all_term_head_tail (TApp u1 u2)) as [t [l H]].
+      eapply lu_red.
+      + apply rt1n_refl.
+      + apply H.
+      +
+
+    ; intros u ; remember (all_terms u).
+    - intros Hlen. inversion Hlen.
+      destruct l.
+      + exfalso. apply (all_terms_non_empty _ Heql).
+      + simpl in H0. discriminate H0.
+    - destruct u.
+      + intros H. apply lu_var.
+      +
+
+End LeftmostUppermost.
+ *)
+
+Inductive StronglyNormalizing : term -> Prop :=
+| SN_Step :
+    forall u : term,
+      (forall v : term, u --> v -> StronglyNormalizing v) ->
+      StronglyNormalizing u.
+
+
+Lemma sn_rescope :
+  forall (u : term) (n : nat), StronglyNormalizing u <-> StronglyNormalizing (rescope u n).
+Proof.
+
+  intros u n. split.
+  - intros Hu. generalize dependent n.
+    induction Hu.
+    intros n. apply SN_Step.
+    * intros n0 G.
+      apply rescope_reduction in G.
+      destruct G as [v [Gr Gred]].
+      rewrite Gr. apply H0. assumption.
+  - intros Hu.
+    remember (rescope u n). generalize dependent n. generalize u.
+    induction Hu.
+    intros v n Hv. apply SN_Step. intros w Hw.
+    apply H0 with (rescope w n) n. rewrite Hv.
+    apply rescope_congr. assumption. reflexivity.
+Qed.
+
+Lemma sn_subst :
+  forall (u : term) (k n : nat),
+    StronglyNormalizing u <-> StronglyNormalizing ([k := TVar n]u).
+Proof.
+  intros u k n. split.
+  - intros Hu. generalize dependent n. generalize dependent k.
+    induction Hu. intros k n. apply SN_Step.
+    intros v Hv.
+    destruct (subst_reduction_inversion _ _ _ _ Hv) as [w [Hw Hr]].
+    rewrite Hw. apply H0. assumption.
+  - intros Hu. remember ([k := TVar n]u).
+    generalize dependent n. generalize dependent k. generalize dependent u.
+    induction Hu. intros v k n Hv. apply SN_Step.
+    intros w Hw. apply H0 with (v:=[k := TVar n]w) (k:=k) (n:=n).
+    rewrite Hv. apply subst_reduction. assumption. reflexivity.
+Qed.
+
+
+Lemma sn_sub_app1 :
+  forall (u v : term), StronglyNormalizing (TApp u v) -> StronglyNormalizing u.
+Proof.
+  intros u v H.
+  remember (TApp u v).
+  generalize dependent v. generalize dependent u.
+  induction H.
+  + intros u0 v0 Heq.
+    apply SN_Step. intros w0 Hu0w0.
+    apply H0 with (v:=TApp w0 v0) (v0:=v0).
+    rewrite Heq. apply b_app1. assumption. reflexivity.
+Qed.
+
+
+Module SimpleType.
+  Inductive ty : Set :=
+  | TBase : ty
+  | TArrow : ty -> ty -> ty.
+
+  Module Context.
+    Definition t := list ty.
+
+    Definition add (c : t) (typ : ty) :=
+      (typ :: c)%list.
+
+    Definition find (c : t) (n : nat) :=
+      List.nth n c.
+
+    Inductive MapsTo : t -> nat -> ty -> Prop :=
+    | MT_Head :
+        forall (c : t) (T : ty),
+          MapsTo (T :: c)%list 0 T
+    | MT_Tail :
+        forall (c : t) (n : nat) (T O : ty),
+          MapsTo c n T ->
+          MapsTo (O :: c)%list (S n) T.
+  End Context.
+
+
+  Inductive typing : Context.t -> term -> ty -> Prop :=
+  | TAxiom :
+      forall (gamma : Context.t) (n : nat) (T : ty),
+        Context.MapsTo gamma n T -> typing gamma (TVar n) T
+  | TArrowElim :
+      forall (gamma : Context.t) (u v : term) (U V : ty),
+        typing gamma u (TArrow U V) ->
+        typing gamma v U ->
+        typing gamma (TApp u v) V
+  | TArrowIntro :
+      forall (gamma : Context.t) (u : term) (U V : ty),
+        typing (Context.add gamma U) u V ->
+        typing gamma (TAbstr u) (TArrow U V).
+
+
+  Inductive reductible_arrow (Pdom Papp : term->Prop) : term->Prop :=
+  | RAArrow :
+      forall (u : term),
+        (forall (v : term),  Pdom v -> Papp (TApp u v)) ->
+        reductible_arrow Pdom Papp u.
+
+  Fixpoint reductible (T : ty) : term -> Prop :=
+    match T with
+      | TBase => StronglyNormalizing
+      | TArrow U V => reductible_arrow (reductible U) (reductible V)
+    end.
+
+  Inductive neutral : term -> Prop :=
+  | NVar : forall (n : nat), neutral (TVar n)
+  | NApp : forall (u1 u2 : term), neutral (TApp u1 u2).
+
+
+  Definition cr1_def (T : ty) :=
+    forall (u : term),  reductible T u -> StronglyNormalizing u.
+
+  Definition cr2_def (T : ty) :=
+    forall (u u' : term),
+      u --> u' ->
+      reductible T u ->
+      reductible T u'.
+
+  Definition cr3_def (T : ty) :=
+    forall (u : term),
+      neutral u ->
+      (forall (v : term),  u --> v -> reductible T v) ->
+      reductible T u.
+
+  Theorem crAll :
+    forall (T : ty), cr1_def T /\ cr2_def T /\ cr3_def T.
+  Proof.
+    induction T ;
+    unfold cr1_def, cr2_def, cr3_def ;
+    (split ; [idtac | split]) ; simpl.
+    - auto.
+    - intros u u'. intros Huu' HSN. inversion HSN ; subst. auto.
+    - intros u _ H. apply SN_Step. assumption.
+
+
+    - intros u G. inversion G ; subst.
+      apply sn_sub_app1 with (TVar 0).
+      destruct IHT1 as [_ [_ cr31]]. unfold cr3_def in cr31.
+      destruct IHT2 as [cr12 [_ _]]. unfold cr1_def in cr12.
+      apply cr12. apply H. apply cr31. apply NVar.
+      intros v contra. inversion contra.
+
+    - unfold cr2_def. simpl.
+      destruct IHT2 as [_ [cr22 _]]. unfold cr2_def in cr22.
+      intros u u' Hr Hu. apply RAArrow.
+      intros v Hv. apply cr22 with (TApp u v). apply b_app1. assumption.
+      inversion Hu. subst. apply H. assumption.
+
+    - destruct IHT1 as [cr11 [cr21 _]].
+      unfold cr1_def in cr11. unfold cr2_def in cr21.
+      destruct IHT2 as [_ [_ cr32]]. unfold cr3_def in cr32.
+      intros u Hnu Hr.
+      apply RAArrow. intros v Hv.
+      assert (Hind := cr11 v Hv). induction Hind.
+      apply cr32. apply NApp. intros w Hw.
+      inversion Hw ; subst.
+      + apply Hr in H4. inversion H4 ; subst. apply H1. assumption.
+      + apply H0. assumption. apply cr21 with u0 ; assumption.
+      + inversion Hnu.
+  Qed.
+
+  Lemma cr1 : forall (T : ty), cr1_def T.
+  Proof. intros T. destruct (crAll T) as [H1 _]. assumption. Qed.
+
+  Lemma cr2 : forall (T : ty), cr2_def T.
+  Proof. intros T. destruct (crAll T) as [_ [H2 _]]. assumption. Qed.
+
+  Lemma cr3 : forall (T : ty), cr3_def T.
+  Proof. intros T. destruct (crAll T) as [_ [_ H3]]. assumption. Qed.
+
+  Lemma cr3' : forall (T : ty) (n : nat),  reductible T (TVar n).
+  Proof. intros T n. apply cr3. apply NVar. intros v Hcontra. inversion Hcontra. Qed.
+
+  Lemma substRed :
+    forall (u : term) (U V : ty),
+      reductible V u ->
+      (forall (v : term), reductible U v -> reductible V ([0 := v]u) ) ->
+      reductible (TArrow U V) (TAbstr u).
+  Proof.
+    intros u U V Hred H.
+    simpl. apply RAArrow.
+    assert (Hind := cr1 V u Hred).
+    induction Hind.
+    intros v Hv.
+    assert (Hind2 := cr1 U v Hv).
+    induction Hind2.
+    apply cr3. apply NApp.
+    assert (Hcr2 := cr2). unfold cr2_def in Hcr2.
+    intros w Hw. inversion Hw ; subst.
+    - inversion H7 ; subst. apply H1 ; try assumption.
+      + apply Hcr2 with u ; assumption.
+      + intros z Hz.
+        apply Hcr2 with ([0 := z]u). apply subst_reduction.
+        assumption. apply H. assumption.
+    - apply H3. assumption. apply Hcr2 with u0 ; assumption.
+    - apply H. assumption.
+  Qed.
+
+
+  Lemma subst_rescope_red :
+    forall (U : ty) (u : term),
+      (forall (k n : nat), reductible U u <-> reductible U ([k := TVar n]u))
+   /\ (forall (n : nat), reductible U u <-> reductible U (rescope u n)).
+  Proof.
+    induction U.
+    - simpl. intros u. split. apply sn_subst. apply sn_rescope.
+    - intros u. split.
+      intros k n ; split.
+      + simpl. intro H. inversion H ; subst.
+        apply RAArrow. intros v.
+        intro G. rewrite <- Parallel.subs_rescope with k v (TVar n).
+        destruct (IHU1 v) as [_ HU1].
+        destruct (IHU2 (TApp u (rescope v k))) as [HU2 _].
+        simpl in HU2. rewrite <- HU2.
+        apply H0. rewrite <- HU1. assumption.
+      + simpl. intro H. inversion H ; subst.
+        apply RAArrow. intros v G.
+        destruct (IHU1 v) as [HU1 _].
+        destruct (IHU2 (TApp u v)) as [HU2 _].
+        rewrite HU2. simpl. apply H0.
+        rewrite <- HU1. assumption.
+      + intros n. split. intro H.
+        remember (rescope u n).
+        assert (M := H).
+        apply cr1 in H. rewrite (sn_rescope _ n) in H.
+        rewrite <- Heqt in H.
+        generalize dependent n. generalize dependent u.
+        induction H. intros v M k K.
+        destruct u eqn:Eq.
+        * apply cr3'.
+        * apply cr3. apply NApp.
+          intros w Hw.
+          rewrite K in Hw. destruct (rescope_reduction _ _ _ Hw) as [o [Ho Hr]].
+          apply H0 with o k. rewrite K. assumption.
+          assert (Hcr2 := cr2). unfold cr2_def in Hcr2.
+          apply Hcr2 with v ; assumption. assumption.
+        * assert (Hcr2 := cr2). unfold cr2_def in Hcr2.
+          apply substRed.
+
+          assert (reductible U2 (TApp v (TVar k))).
+          simpl in M. inversion M ; subst. apply H1. apply cr3'.
+          destruct (IHU2 t) as [GU2 _].
+          destruct (IHU2 (TApp v (TVar k))) as [_ HU2].
+          assert (reductible U2 (rescope (TApp v (TVar k)) k)).
+          apply HU2. assumption.
+          simpl in H2. rewrite <- K in H2.
+          assert (leb k k = true). apply leb_correct. omega.
+          rewrite H3 in H2.
+          rewrite GU2. apply Hcr2 with (TApp (TAbstr t) (TVar (S k))).
+          apply b_red. assumption.
+
+          intros w Hw.
+          apply Hcr2 with (TApp (TAbstr t) w).
+          apply b_red.
+          destruct (IHU2 (TApp (rescope v k) w)) as [HU2 _].
+          assert (GU2 := HU2 k k).
+          simpl in GU2.
+          rewrite Parallel.subs_rescope in GU2.
+          rewrite <- K in GU2.
+          rewrite GU2.
+          simpl in M. inversion M ; subst.
+          apply H1.
+          destruct (IHU1 w) as [HU1 _].
+          rewrite <- HU1. assumption.
+        * intros H. simpl. apply RAArrow.
+          intros v Hv.
+          destruct (IHU2 (TApp u v)) as [_ HU2].
+          rewrite HU2.
+          inversion H ; subst.
+          simpl. apply H0.
+          destruct (IHU1 v) as [_ HU1].
+          rewrite <- HU1. assumption.
+  Qed.
+
+
+
+  Lemma rescope_red :
+    forall (U : ty) (u : term) (n : nat),
+      reductible U u <-> reductible U (rescope u n).
+  Proof.
+    intros U u. destruct (subst_rescope_red U u) as [_ P]. exact P.
+  Qed.
+
+  Require Export Coq.FSets.FMapList.
+  Require Export Coq.Structures.OrderedTypeEx.
+
+  Module NatMap := FMapList.Make (Nat_as_OT).
+
+  Definition rescope_parallel (l : list term) :=
+    (TVar 0 :: (List.map (fun t => rescope t 0) l))%list.
+
+  Fixpoint subst_parallel (l : list term) (u : term) :=
+    match u with
+      | TVar n => List.nth n l (TVar n)
+      | TApp u1 u2 =>
+        TApp (subst_parallel l u1) (subst_parallel l u2)
+      | TAbstr u => TAbstr (subst_parallel (rescope_parallel l) u)
+    end.
+
+  Fixpoint replace (l : list term) (n : nat) (u : term) :=
+   (match l with
+      | nil => nil
+      | a :: t =>
+        match n with
+          | 0 => u :: t
+          | S p => a :: replace t p u
+        end
+    end)%list.
+
+  Inductive AssocSubst : Context.t -> list term -> Prop :=
+  | ASEmpty : AssocSubst nil nil
+  | ASCons : forall (U : ty) (Tl : Context.t) (u : term) (tl : list term),
+               reductible U u ->
+               AssocSubst Tl tl ->
+               AssocSubst (U :: Tl)%list (u :: tl)%list.
+
+  Lemma nth_replace_eq :
+    forall (s : list term) (n : nat) (u v : term),
+      n < List.length s ->
+      List.nth n (replace s n u) v = u.
+  Proof.
+    induction s.
+    - intros n u v H. inversion H.
+    - intros n u v H.
+      destruct n.
+      + reflexivity.
+      + simpl. rewrite IHs. reflexivity. simpl in H. omega.
+  Qed.
+
+  Lemma nth_replace_neq :
+    forall (s : list term) (p q : nat) (u v : term),
+      p <> q ->
+      List.nth p (replace s q u) v = List.nth p s v.
+  Proof.
+    induction s.
+    - intros. simpl. reflexivity.
+    - intros. simpl.
+      destruct q ; destruct p.
+      + contradict H. reflexivity.
+      + simpl. reflexivity.
+      + simpl. reflexivity.
+      + simpl. apply IHs. omega.
+  Qed.
+
+
+
+  Lemma assoc_mapsto :
+    forall (gamma : Context.t) (sub : list term) (n : nat) (U : ty),
+      AssocSubst gamma sub ->
+      Context.MapsTo gamma n U ->
+      exists (u : term), reductible U u /\
+                         (forall k : nat,  List.nth n sub (TVar k) = u).
+  Proof.
+    induction gamma.
+    - intros sub n U _ H. inversion H.
+    - intros sub n U Hassoc Hmaps.
+      destruct n.
+      + inversion Hmaps ; subst.
+        inversion Hassoc ; subst.
+        exists u. split. assumption. simpl. reflexivity.
+      + inversion Hassoc; subst. simpl.
+        inversion Hmaps ; subst.
+        apply IHgamma ; assumption.
+  Qed.
+
+  Lemma assoc_rescope :
+    forall (gamma : Context.t) (sub : list term) (U : ty),
+      AssocSubst gamma sub ->
+      AssocSubst (Context.add gamma U) (rescope_parallel sub).
+  Proof.
+    intros gamma. unfold Context.add, rescope_parallel.
+    intros sub U Hassoc.
+    apply ASCons. apply cr3'.
+    generalize dependent sub.
+    induction gamma.
+    - intros sub Hassoc. inversion Hassoc. simpl. apply ASEmpty.
+    - intros sub Hassoc. inversion Hassoc ; subst.
+      simpl. apply ASCons. apply rescope_red. assumption.
+      apply IHgamma. assumption.
+  Qed.
+
+
+  Lemma S_iterate :
+    forall (n : nat) (A : Set) (f : A -> A) (a : A),
+      iterate (S n) f a = f (iterate n f a).
+  Proof. intros. reflexivity. Qed.
+
+
+  Lemma iterate_S :
+    forall (n : nat) (A : Set) (f : A -> A) (a : A),
+      iterate (S n) f a = iterate n f (f a).
+  Proof.
+    induction n.
+    - reflexivity.
+    - intros A f a. replace (iterate (S (S n)) f a) with (f (iterate (S n) f a)).
+      pattern (iterate (S n) f a) at 1. rewrite IHn. simpl. reflexivity.
+      reflexivity.
+  Qed.
+
+  Lemma existing_nth_map :
+    forall (sub : list term) (n : nat) (r : term),
+      (forall (u : term), List.nth n sub u = r) ->
+      (forall (u : term) (f : term -> term),  List.nth n (List.map f sub) u = f r).
+  Proof.
+    induction sub.
+    - intros n r H.
+      assert (G := H (TVar 0)).
+      assert (TVar 0 = r). rewrite <- G. simpl. destruct n ; reflexivity.
+      assert (K := H (TVar 1)).
+      assert (TVar 1 = r). rewrite <- K. simpl. destruct n ; reflexivity.
+      rewrite <- H0 in H1. discriminate H1.
+    -intros n r H.
+     destruct n.
+     + simpl. simpl in H. assert (G := H (TVar 0)). rewrite G.
+       reflexivity.
+     + simpl. apply IHsub. simpl in H. exact H.
+  Qed.
+
+  Definition it_rescope (k n : nat) (u : term)  :=
+    iterate n (fun (t : term) => rescope t k) u.
+
+  Lemma nth_rescope_parallel :
+    forall (sub : list term) (n k : nat) (u : term),
+      n < k -> List.nth n (iterate k rescope_parallel sub) u = TVar n.
+  Proof.
+    intros sub n k. generalize dependent sub. generalize dependent n.
+    induction k.
+    - intros n sub u H. inversion H.
+    - intros n sub u H.
+      inversion H. simpl.
+      destruct k. reflexivity.
+      + rewrite existing_nth_map with (r := TVar k). reflexivity.
+        intros w. apply IHk. omega.
+      + subst.
+        destruct n.
+        * reflexivity.
+        * simpl. rewrite existing_nth_map with (r := TVar n).
+          reflexivity.
+          intros w. apply IHk. omega.
+  Qed.
+
+  Lemma nth_rescope_parallel' :
+    forall (sub : list term) (n k : nat) (u : term),
+      n >= k ->
+      List.nth n (iterate k rescope_parallel sub) u
+      = List.nth (n - k) (List.map (it_rescope 0 k) sub) u.
+  Proof.
+    intros sub n k. generalize dependent n. generalize dependent sub.
+    induction k.
+    - intros sub n. replace (n - 0) with n. simpl. generalize dependent n.
+      induction sub ; intros n u H.
+      + simpl. destruct n ; reflexivity.
+      + simpl. destruct n. reflexivity. apply IHsub. omega.
+      + omega.
+    - intros sub n u H. rewrite iterate_S. rewrite IHk.
+      simpl. assert (n - k <> 0). omega.
+      destruct (n - k) eqn:Eq. contradict H0. reflexivity.
+      assert ((n - S k) = n0). omega. rewrite H1.
+      unfold it_rescope.
+      rewrite List.map_map.
+      remember (fun v : term => rescope v 0).
+      remember (fun x : term => iterate k t (rescope x 0)) as f.
+      remember (fun t0 : term => rescope (iterate k t t0) 0) as g.
+      rewrite List.map_ext with term term f g sub. rewrite Heqg. rewrite Heqt. simpl.
+       reflexivity.
+       intros z. rewrite Heqf. rewrite Heqg.
+       replace (rescope z 0) with (t z). rewrite <- iterate_S.
+       simpl. rewrite Heqt. reflexivity. rewrite Heqt. reflexivity.
+       omega.
+  Qed.
+
+
+  Hint Unfold it_rescope.
+
+  Lemma rescope_iterate_var :
+    forall (n k p : nat),
+      k <= p -> it_rescope k n (TVar p) = TVar (p + n).
+  Proof.
+    unfold it_rescope.
+    induction n.
+    - simpl. auto.
+    - intros. rewrite iterate_S. simpl.
+      assert (G := H). apply leb_correct in H. rewrite H.
+      rewrite IHn. replace (S p + n) with (p + S n). reflexivity.
+      omega. omega.
+  Qed.
+
+  Lemma rescope_iterate_var' :
+    forall (n k p : nat),
+      k > p -> it_rescope k n (TVar p) = TVar p.
+  Proof.
+    unfold it_rescope.
+    induction n.
+    - simpl. reflexivity.
+    - intros. rewrite iterate_S. simpl.
+      assert (G := H). apply leb_correct_conv in H. rewrite H.
+      rewrite IHn. reflexivity. assumption.
+  Qed.
+
+
+  Lemma rescope_iterate_app :
+    forall (n k : nat) (u1 u2 : term),
+      it_rescope k n (TApp u1 u2) =
+      TApp (it_rescope k n u1) (it_rescope k n u2).
+  Proof.
+    unfold it_rescope.
+    induction n.
+    - simpl. reflexivity.
+    - simpl. intros. rewrite IHn. simpl. reflexivity.
+  Qed.
+
+  Lemma rescope_iterate_abs :
+    forall (n k : nat) (u : term),
+      it_rescope k n (TAbstr u) =
+      TAbstr (it_rescope (S k) n u).
+  Proof.
+    unfold it_rescope.
+    induction n.
+    - simpl. reflexivity.
+    - simpl. intros. rewrite IHn. simpl. reflexivity.
+  Qed.
+
+
+
+
+  Lemma subst_rescope_iterate :
+    forall (k p s : nat) (u v : term),
+      p <= s -> s <= p + k ->
+      [s := v](it_rescope p (S k) u) =
+               it_rescope p    k  u.
+  Proof.
+    intros k p s u.
+    generalize dependent s. generalize dependent p. generalize dependent k.
+    induction u.
+    - simpl. intros k p s v G K.
+      destruct (le_lt_dec p n).
+      + rewrite rescope_iterate_var.
+        rewrite rescope_iterate_var.
+        simpl. assert (nat_compare s (n + S k) = Lt).
+        apply nat_compare_lt. omega. rewrite H.
+        replace (pred (n + S k)) with (n + k).
+        reflexivity. omega. assumption. assumption.
+      + rewrite rescope_iterate_var'.
+        rewrite rescope_iterate_var'.
+        simpl. assert (nat_compare s n = Gt).
+        apply nat_compare_gt. omega.
+        rewrite H. reflexivity. assumption. assumption.
+    - intros k p s v G K. simpl.
+      repeat (rewrite rescope_iterate_app). simpl.
+      rewrite IHu1. rewrite IHu2. reflexivity.
+      assumption. assumption.
+      assumption. assumption.
+    - intros k p s v G K. simpl.
+      repeat (rewrite  rescope_iterate_abs). simpl.
+      rewrite IHu. reflexivity.
+      omega. omega.
+  Qed.
+
+  Lemma rescope_it_rescope :
+    forall (u : term) (i p k : nat),
+      p <= i ->
+      rescope (it_rescope k i u) k = rescope (it_rescope k i u) (k + p).
+  Proof.
+    induction u.
+    - intros i p k H.
+      destruct (le_lt_dec k n).
+      + rewrite rescope_iterate_var. simpl.
+        rewrite leb_correct. rewrite leb_correct. reflexivity.
+        omega. omega. omega.
+      + rewrite rescope_iterate_var'. simpl.
+        rewrite leb_correct_conv. rewrite leb_correct_conv. reflexivity.
+        omega. omega. omega.
+    - intros. rewrite rescope_iterate_app. simpl.
+      rewrite IHu1 with i p k. rewrite IHu2 with i p k.
+      reflexivity. assumption. assumption.
+    - intros i p k H. rewrite rescope_iterate_abs. simpl.
+      rewrite IHu with i p (S k). simpl. reflexivity.
+      omega.
+  Qed.
+
+
+  Lemma rescope_parallel_iterate_var :
+    forall (p k : nat) (sub : list term),
+      k < p ->
+      subst_parallel (iterate p rescope_parallel sub) (TVar k) = TVar k.
+  Proof. intros. simpl. rewrite nth_rescope_parallel. reflexivity. assumption. Qed.
+
+  Lemma rescope_parallel_iterate_var' :
+    forall (p k : nat) (sub : list term),
+      p <= k ->
+      subst_parallel (iterate p rescope_parallel sub) (TVar k)
+      = it_rescope 0 p (List.nth (k - p) sub (TVar (k - p))).
+  Proof.
+    intros. simpl. rewrite nth_rescope_parallel'.
+    replace (TVar k) with (it_rescope 0 p (TVar (k - p))).
+    rewrite List.map_nth. reflexivity.
+    rewrite rescope_iterate_var.
+    replace (k - p + p) with k. reflexivity.
+    omega. omega. omega.
+  Qed.
+
+  Lemma subst_rescope_parallel_var :
+    forall (p k : nat) (sub : list term),
+      subst_parallel (rescope_parallel (iterate p rescope_parallel sub))
+                     (rescope (TVar k) p)
+      = rescope (subst_parallel (iterate p rescope_parallel sub) (TVar k)) p.
+  Proof.
+    intros p k sub.
+    destruct (le_lt_dec p k).
+    - rewrite rescope_parallel_iterate_var'.
+      simpl. rewrite leb_correct. rewrite <- S_iterate.
+      rewrite rescope_parallel_iterate_var'.
+      assert(G := rescope_it_rescope).
+      unfold it_rescope. unfold it_rescope in G.
+      rewrite S_iterate. replace (S k - S p) with (k - p).
+      rewrite G with (p := p). replace (0 + p) with p.
+      reflexivity. omega. omega. omega. omega. assumption. assumption.
+    - rewrite rescope_parallel_iterate_var. simpl.
+      rewrite leb_correct_conv.
+      rewrite <- S_iterate. rewrite rescope_parallel_iterate_var. reflexivity.
+       omega. assumption. assumption.
+  Qed.
+
+  Lemma subst_rescope_parallel_iterate_var :
+    forall (i p : nat) (k : nat) (sub : list term),
+      subst_parallel (iterate (i + p) rescope_parallel sub)
+                     (it_rescope p i (TVar k) )
+      = it_rescope p i (subst_parallel (iterate p rescope_parallel sub) (TVar k)).
+  Proof.
+    induction i.
+    - unfold it_rescope. simpl. reflexivity.
+    - intros p k sub.
+      replace (it_rescope p (S i) (TVar k))
+      with (rescope (it_rescope p i (TVar k)) (i + p)).
+      destruct (le_lt_dec p k).
+      + simpl.
+        rewrite rescope_iterate_var. rewrite subst_rescope_parallel_var.
+        rewrite <- rescope_iterate_var with (k := p). rewrite IHi.
+        unfold it_rescope. simpl.
+        assert (G := rescope_it_rescope). unfold it_rescope in G.
+        rewrite G with (p := i). replace (i + p) with (p + i).
+        reflexivity. omega. omega. assumption. assumption.
+      + rewrite rescope_iterate_var'.
+        rewrite rescope_parallel_iterate_var.
+        simpl. rewrite leb_correct_conv.
+        rewrite <- S_iterate. rewrite rescope_parallel_iterate_var.
+        rewrite rescope_iterate_var'. reflexivity.
+        omega. omega. omega. omega. omega.
+      + assert (G := rescope_it_rescope).
+        rewrite plus_comm. rewrite <- G.
+        unfold it_rescope. simpl. reflexivity.
+        apply le_refl.
+  Qed.
+
+  Lemma subst_rescope_parallel_iterate :
+    forall (u : term) (i p : nat) (sub : list term),
+      subst_parallel (iterate (i + p) rescope_parallel sub)
+                     (it_rescope p i u )
+      = it_rescope p i (subst_parallel (iterate p rescope_parallel sub) u).
+  Proof.
+    induction u.
+    - intros i p sub. apply subst_rescope_parallel_iterate_var.
+    - intros i p sub. simpl.
+      repeat (rewrite rescope_iterate_app).
+      simpl. rewrite IHu1. rewrite IHu2. reflexivity.
+    - intros i p sub. simpl.
+      repeat (rewrite rescope_iterate_abs). simpl.
+      rewrite <- S_iterate. replace (S (i + p)) with (i + S p).
+      rewrite IHu. simpl. reflexivity. omega.
+  Qed.
+
+  Lemma iterate_rescope_parallel_length :
+    forall (k : nat) (sub : list term),
+      length (iterate k rescope_parallel sub) = k + length sub.
+  Proof.
+    induction k.
+    - simpl. reflexivity.
+    - intros sub. simpl. rewrite List.map_length.
+      rewrite IHk. reflexivity.
+  Qed.
+
+  Lemma replace_rescope_parallel :
+    forall (sub : list term) (k : nat) (v : term),
+      replace (rescope_parallel sub) (S k) (rescope v 0) =
+      rescope_parallel (replace sub k v).
+  Proof.
+    induction sub.
+    - intros k v. simpl. unfold rescope_parallel. simpl. reflexivity.
+    - intros k v.
+      destruct k.
+      + simpl. unfold rescope_parallel. simpl. reflexivity.
+      + simpl.
+        assert (G := IHsub k v).
+        simpl in G. unfold rescope_parallel in G.
+        inversion G ; subst. rewrite H0.
+        unfold rescope_parallel. simpl. reflexivity.
+  Qed.
+
+  Lemma subst_subst_parallel :
+    forall (u v : term) (sub : list term) (k : nat),
+      rescope ([k := v](subst_parallel (iterate (S k) rescope_parallel sub) u)) k =
+      subst_parallel (replace (iterate (S k) rescope_parallel sub) k (rescope v k)) u.
+  Proof.
+    induction u.
+    - intros v sub k.
+      destruct (le_lt_dec n k).
+      + rewrite rescope_parallel_iterate_var.
+        inversion l. remember (S k).
+        * simpl. replace (nat_compare k k) with Eq.
+          rewrite nth_replace_eq. reflexivity.
+          rewrite iterate_rescope_parallel_length. omega.
+          symmetry. apply nat_compare_eq_iff. reflexivity.
+        * remember (S m). remember (S n0).
+          simpl. replace (nat_compare n0 n) with Gt.
+          rewrite nth_replace_neq. rewrite nth_rescope_parallel.
+          simpl. rewrite leb_correct_conv. reflexivity.
+          omega. omega. omega. symmetry. rewrite <- nat_compare_gt. omega.
+        * omega.
+      + replace (TVar n) with (it_rescope k 1 (TVar (n - 1))).
+        replace (S k) with (1 + k).
+        rewrite subst_rescope_parallel_iterate.
+        unfold it_rescope.
+        remember (1 + k). simpl. rewrite Parallel.subs_rescope.
+        rewrite leb_correct. simpl.
+        rewrite nth_replace_neq. rewrite Heqn0. simpl.
+        remember (fun t => rescope t 0).
+        replace (TVar (S (n - 1))) with (t (TVar (n - 1))).
+        rewrite List.map_nth.
+        rewrite nth_rescope_parallel'.
+        replace (TVar (n - 1)) with (it_rescope 0 k (TVar (n - 1 - k))).
+        rewrite List.map_nth. rewrite Heqt.
+        rewrite rescope_it_rescope with (p := k). replace (0 + k) with k.
+        reflexivity.
+        omega. omega.
+        rewrite rescope_iterate_var. replace (n - 1 - k + k) with (n - 1).
+        reflexivity. omega. omega. omega. rewrite Heqt. simpl. reflexivity.
+        omega. omega. omega.
+        unfold it_rescope. simpl. rewrite leb_correct.
+        replace (S (n - 1)) with n. reflexivity.
+        omega. omega.
+    - intros v sub k.
+      remember (S k). simpl. rewrite Heqn.
+      rewrite IHu1. rewrite IHu2. reflexivity.
+    - intros v sub k.
+      remember (S k). simpl.
+      rewrite Heqn. rewrite <- S_iterate. rewrite IHu.
+      rewrite S_iterate.
+      rewrite iterate_S. rewrite <- Parallel.rescope_comm.
+      rewrite replace_rescope_parallel. reflexivity.
+      omega.
+  Qed.
+
+  Lemma map_rescope_assoc_subst :
+    forall (sub : list term) (gamma : Context.t),
+      AssocSubst gamma sub ->
+      AssocSubst gamma (List.map (fun t => rescope t 0) sub).
+  Proof.
+    induction sub.
+    - simpl. auto.
+    - intros gamma H. inversion H ; subst. simpl.
+      apply ASCons. rewrite <- rescope_red. assumption.
+      apply IHsub. assumption.
+  Qed.
+
+  Theorem typing_implies_reductible :
+    forall (gamma : Context.t) (u : term) (U : ty),
+      typing gamma u U ->
+      forall (sub : list term),
+        AssocSubst gamma sub ->
+        reductible U (subst_parallel sub u).
+  Proof.
+    intros gamma u U Hderiv. induction Hderiv.
+    - intros sub G. simpl.
+      assert (H1 := assoc_mapsto gamma sub n T).
+      destruct H1 as [u [Hru Hln]] ; try assumption.
+      rewrite Hln. assumption.
+    - intros sub Hassoc. simpl.
+      assert (H1 := IHHderiv1 sub Hassoc).
+      simpl in H1. inversion H1 ; subst.
+      apply H. apply IHHderiv2. assumption.
+    - intros sub Hassoc. simpl. apply substRed.
+      apply IHHderiv. apply assoc_rescope. assumption.
+      intros v Hv.
+      rewrite rescope_red. rewrite subst_subst_parallel.
+      apply IHHderiv. simpl.
+      apply ASCons. rewrite <- rescope_red. assumption.
+      apply map_rescope_assoc_subst. assumption.
+  Qed.
